\documentclass[a4paper, 100pt]{scrartcl}

\usepackage{amsmath}
\usepackage{amssymb}
\usepackage{geometry}
\geometry{
	left=3cm,
	right=3cm,
	top=2cm,
	bottom=4cm,
	bindingoffset=5mm
}

\begin{document}
	
	\textbf{Y = ($\overline{\textbf{A}}$+B)C + $\overline{\textbf{ACD}}$} 
	\\
	\\
	\textbf{Y = ($\overline{\textbf{A} \oplus\textbf{C}}$)\textbf{AC} + $\overline{\textbf{D}}$} 
	\\
	\\
	\textbf{Y = ($\overline{\textbf{C}}$D + \textbf{BD}) $\oplus$ A}
	\\
	\\
	\textbf{Y = ($\overline{\overline{\textbf{B}}+\textbf{D}}$)C $\oplus$ AB}
	\\
	\\
	\textbf{Y = $\overline{\overline{\textbf{AB}}\oplus \textbf{AC}}$}
	\\
	\\
	\textbf{Y = ($\overline{\textbf{A}}\oplus\overline{\textbf{C}}$)D $\oplus$ ABC}
	\\
	\\
	\textbf{Y = ($\overline{\overline{\textbf{D}}\textbf{B}}$ + A$\overline{\textbf{C}}$) $\oplus$ CD}
	\\
	\\
	\textbf{Y = (C + A$\overline{\textbf{DC}}$) $\oplus$ B}
\end{document}